Update SSA to use the general definitions and utilities
Removed some duplicated definitions after including the Definitions.dfy
and  Util.dfy and fixed some issues related to the differences in
definitions, for example that Expression is no longer a string, so
seq<Expression> can no longer be assigned with a seq<Variable> (we now
have a function to convert such a sequence of variables to a sequence of
expressions).

SSA.dfy
@@ -1,9 +1,6 @@
-datatype Statement = Assignment(LHS : seq<Variable>, RHS : seq<Expression>) | Skip | SeqComp(S1 : Statement, S2 : Statement) | 
-		IF(B0 : BooleanExpression, Sthen : Statement, Selse : Statement) | DO(B : BooleanExpression, S : Statement) |
-		LocalDeclaration(L : seq<Variable>, S0 : Statement)
-type Variable = string
-type Expression = string
-type BooleanExpression = string
+include "Definitions.dfy"
+//include "Substitutions.dfy"
+include "Util.dfy"
 
 class VariablesSSA {
 
@@ -257,63 +254,12 @@ method Main()
 }
 
 
-predicate method ValidAssignment(str : string)
-{
-	true // check ":=" with same-length lists to its left and right, the former of distinct variable names and the right of expressions
-}
-
-predicate Valid(stmt: Statement)
-{
-	match stmt {
-		case Skip => true
-		case Assignment(LHS, RHS) => |LHS| == |RHS|
-		case SeqComp(S1,S2) => Valid(S1) && Valid(S2)
-		case IF(B,Sthen,Selse) => Valid(Sthen) && Valid(Selse)
-			//(forall state: State :: B.requires(state) && B(state).Bool?) && 
-			//Valid(Sthen) && Valid(Selse)
-		case DO(B,S) => Valid(S)
-			//(forall state: State :: B.requires(state) && B(state).Bool?) && Valid(S)
-		case LocalDeclaration(L,S) => Valid(S)
-	} 
-	//&&
-	//forall state1: State, P: Predicate  :: P.requires(state1)
-
-}
-
 predicate ValidVsSSA(vsSSA: VariablesSSA) reads vsSSA
 {
 	vsSSA != null && vsSSA.n >= 1 && (forall v :: v in vsSSA.instancesOf ==> |vsSSA.instancesOf[v]| >= 1)
 	&& (forall i :: i in vsSSA.variableOf ==> vsSSA.variableOf[i] in vsSSA.instancesOf && i in vsSSA.instancesOf[vsSSA.variableOf[i]])
 	&& (forall v :: v in vsSSA.instancesOf ==> (forall i :: i in vsSSA.instancesOf[v] ==> i in vsSSA.variableOf && vsSSA.variableOf[i] == v))
 	&& (forall v :: v in vsSSA.instancesOf ==> vsSSA.existsInstance(v)) && (forall i :: i in vsSSA.variableOf ==> vsSSA.existsVariable2(i))
-}
-
-method digitToString(num: int) returns (str: string)
-	requires num >= 0 && num <= 9
-{
-	if num == 0 { str := "0"; }
-	else if num == 1 { str := "1"; }
-	else if num == 2 { str := "2"; }
-	else if num == 3 { str := "3"; }
-	else if num == 4 { str := "4"; }
-	else if num == 5 { str := "5"; }
-	else if num == 6 { str := "6"; }
-	else if num == 7 { str := "7"; }
-	else if num == 8 { str := "8"; }
-	else if num == 9 { str := "9"; }
-}
-
-
-method intToString(num: int) returns (str: string)
-	requires num >= 0
-{
-	if num >= 0 && num <= 9 { str := digitToString(num); }
-	else
-	{
-		var digitStr := digitToString(num % 10);
-		var str' := intToString(num / 10);
-		str := str' + digitStr;
-	}
 }
 
  method freshInit(vars : seq<Variable>, ghost allVars : set<Variable>, vsSSA : VariablesSSA) returns (res: seq<Variable>)
@@ -334,57 +280,6 @@ method intToString(num: int) returns (str: string)
 
 		res := [newInstance] + res';
 	}
-}
-
-function method def(S : Statement) : set<Variable> // FIXME: make it return a set
-//	ensures def(S) == {"i","sum","prod"};
-{
-	match S {
-		case Assignment(LHS,RHS) => setOf(LHS) // FIXME
-		case Skip => {}
-		case SeqComp(S1,S2) => def(S1) + def(S2)
-		case IF(B0,Sthen,Selse) => def(Sthen) + def(Selse)
-		case DO(B,S) => def(S)
-		case LocalDeclaration(L,S0) => def(S0) - setOf(L)
-	}
-}
-
-function method ddef(S : Statement) : set<Variable>
-//	ensures ddef(S) == ["i","sum","prod"];
-{
-	match S {
-		case Assignment(LHS,RHS) => setOf(LHS) // FIXME
-		case Skip => {}
-		case SeqComp(S1,S2) => ddef(S1) + ddef(S2)
-		case IF(B0,Sthen,Selse) => ddef(Sthen) * ddef(Selse)
-		case DO(B,S) => {}
-		case LocalDeclaration(L,S0) => ddef(S0) - setOf(L)
-	}
-}
-
-function method input(S : Statement) : set<Variable>
-//	ensures input(S) == ["i","sum","prod"];
-{
-	match S {
-		case Assignment(LHS,RHS) => setOf(LHS) // FIXME (LHS is a sequence of Expression(s), not Variable(s)
-		case Skip => {}
-		case SeqComp(S1,S2) => input(S1) + (input(S2) - ddef(S1)) // right?
-		case IF(B0,Sthen,Selse) => setOf([B0]) + input(Sthen) + input(Selse) // FIXME: variables of B0?
-		case DO(B,S) => setOf([B]) + input(S) // FIXME: variables of B?
-		case LocalDeclaration(L,S0) => input(S0) - setOf(L) // FIXME is the "- L" not redundant?
-	}
-}
-
-function method glob(S : Statement) : set<Variable>
-	//ensures glob(S) == setOf(def(S) + input(S));
-{
-	set v | v in def(S) + input(S)
-}
-
-function method setOf(s : seq<Variable>) : set<Variable>
-	ensures forall v :: v in setOf(s) ==> v in s
-{
-	set x | x in s
 }
 
 
@@ -521,7 +416,8 @@ method SubstitueExpressionSeq(E: seq<Expression>, X: seq<set<Variable>>, XLi: se
 }
 
 method SubstitueBooleanExpression(B: BooleanExpression, X: seq<set<Variable>>, XLi: seq<set<Variable>>) returns (B': BooleanExpression)
-	ensures |B| == |B'|
+// ensures |B| == |B'|
+	ensures B == B' // FIXME: replace with an appropriate call to one of the functions in the new "Substitutions.dfy"
 {
 	B' := B;
 	// TODO - OR!
@@ -572,7 +468,7 @@ method FindIndexOfNum(arr: seq<int>, num: int) returns (i: int)
 	}
 }
 
-method GetNewRHS(indices: seq<int>, E: seq<Expression>, index: int) returns (RHS': seq<Variable>)
+method GetNewRHS(indices: seq<int>, E: seq<Expression>, index: int) returns (RHS': seq<Expression>)
 	requires |indices| == |E|
 	requires index >= 0
 	requires index <= |indices| 
@@ -811,6 +707,7 @@ method {:verify false}OrganizeVariables(vars1: seq<Variable>, vars2: seq<Variabl
 
 method ToSSA(S: Statement, X: seq<Variable>, liveOnEntryX: set<Variable>, liveOnExitX: set<Variable>, Y: set<Variable>, XLs: set<Variable>, vsSSA: VariablesSSA) returns(S': Statement)
 	requires Valid(S)
+	requires (Core(S))
 	requires ValidVsSSA(vsSSA)
 	//requires S.Assignment? ==> setOf(S.LHS) <= (setOf(X) + Y)
 	requires forall i :: i in liveOnEntryX ==> vsSSA.existsVariable2(i)
@@ -843,7 +740,6 @@ method ToSSA(S: Statement, X: seq<Variable>, liveOnEntryX: set<Variable>, liveOn
 		case SeqComp(S1,S2) => S' := SeqCompToSSA(S1, S2, X, liveOnEntryX, liveOnExitX, Y, XLs, vsSSA);
 		case IF(B0,Sthen,Selse) => S' := Skip;//IfToSSA(B0, Sthen, Selse, X, liveOnEntryX, liveOnExitX, Y, XLs, vsSSA);
 		case DO(B,S) => S' := Skip;//DoToSSA(B, S, X, liveOnEntryX, liveOnExitX, Y, XLs, vsSSA);
-		case LocalDeclaration(L,S0) => S' := Skip;
 		case Skip => S' := Skip;
 	}
 }
@@ -1115,6 +1011,7 @@ method {:verify true}SeqCompToSSA(S1: Statement, S2: Statement, X: seq<Variable>
 	// עד לפה התקמפל בערך 40 דקות
 	*/
 	S' := Skip;
+	assume Valid(S');
 }
 
 method {:verify false}IfToSSA(B : BooleanExpression, S1 : Statement, S2 : Statement, X: seq<Variable>, liveOnEntryX: set<Variable>, liveOnExitX: set<Variable>, Y: set<Variable>, XLs: set<Variable>, vsSSA: VariablesSSA) returns (S': Statement)
@@ -1283,7 +1180,8 @@ method {:verify false}IfToSSA(B : BooleanExpression, S1 : Statement, S2 : Statem
 	assert forall i :: i in liveOnExitX' ==> vsSSA.existsVariable2(i);
 	var S1' := ToSSA(S1, X, liveOnEntryX, liveOnExitX', Y, XLs', vsSSA); 
 
-	var XLs'' := XLs' + (glob(S1') - Y);
+	var globS1' := def(S1') + input(S1');
+	var XLs'' := XLs' + (globS1' - Y);
 	temp := setToSeq(XL3i);
 	assert forall i :: i in temp ==> vsSSA.existsVariable2(i);
 	assert forall i :: i in XL4e ==> vsSSA.existsVariable2(i);
@@ -1292,8 +1190,8 @@ method {:verify false}IfToSSA(B : BooleanExpression, S1 : Statement, S2 : Statem
 	assert forall i :: i in liveOnExitX' ==> vsSSA.existsVariable2(i);
 	var S2' := ToSSA(S2, X, liveOnEntryX, liveOnExitX', Y, XLs'', vsSSA);
 
-	var tempAssignment1 := Assignment(XL4fThenSeq + XL5fSeq, XL4t + XL5t);
-	var tempAssignment2 := Assignment(XL4fElseSeq + XL5fSeq, XL4e + XL5e);
+	var tempAssignment1 := Assignment(XL4fThenSeq + XL5fSeq, seqVarToSeqExpr(XL4t + XL5t));
+	var tempAssignment2 := Assignment(XL4fElseSeq + XL5fSeq, seqVarToSeqExpr(XL4e + XL5e));
 	assert Valid(tempAssignment1);
 	assert Valid(tempAssignment2);
 	var tempSeqComp1 := SeqComp(S1', tempAssignment1);
@@ -1436,13 +1334,13 @@ method {:verify false}DoToSSA(B : BooleanExpression, S : Statement, X: seq<Varia
 	var S' := ToSSA(S, X, setOf(liveOnEntryX'), setOf(liveOnExitX'), Y, XLs', vsSSA);
 
 	var tempDO := DO(B', S');
-	var tempAssignment := Assignment(XL2Seq + XL4fSeq, XL2bSeq + XL4bSeq);
+	var tempAssignment := Assignment(XL2Seq + XL4fSeq, seqVarToSeqExpr(XL2bSeq + XL4bSeq));
 	assert Valid(tempDO);
 	assert Valid(tempAssignment);
 	var DO' := SeqComp(tempDO, tempAssignment);
 	assert Valid(DO');
 	//var DO' := SeqComp(DO(B', S'), Assignment(XL2Seq + XL4fSeq, XL2bSeq + XL4bSeq));
-	tempAssignment := Assignment(XL2Seq + XL4fSeq, XL2iSeq + XL4iSeq);
+	tempAssignment := Assignment(XL2Seq + XL4fSeq, seqVarToSeqExpr(XL2iSeq + XL4iSeq));
 	assert Valid(tempAssignment);
 	S'' := SeqComp(tempAssignment, DO');
 	//S'' := SeqComp(Assignment(XL2Seq + XL4fSeq, XL2iSeq + XL4iSeq), DO');
